Updates

generic/Zeta.AppSimulate.Helper.fsti
@@ -17,3 +17,75 @@ val simulate_arity0_leaves_state_unchanged
                     Some? o ==>
                     (let st',_ = Some?.v o in
                      st k = st' k)))
+
+(* equality of two app states *)
+let app_state_feq #adm (st1 st2: app_state adm)
+  = forall (k: app_key adm). {:pattern (st1 k = st2 k)} st1 k = st2 k
+
+val app_state_feq_implies_equal (#adm:_) (st1 st2: app_state adm)
+  : Lemma (requires (app_state_feq st1 st2))
+          (ensures (st1 == st2))
+          [SMTPat (app_state_feq st1 st2)]
+
+(* a correct function call is one which does not fail on the input *)
+let correct #app (fc: appfn_call app)
+  = let fn = appfn fc.fid_c in
+    let rc,_,_ = fn fc.arg_c fc.inp_c in
+    rc = Fn_success
+
+let result #app (fc: appfn_call app{correct fc})
+  = let fn = appfn fc.fid_c in
+    let _,res,_ = fn fc.arg_c fc.inp_c in
+    res
+
+let writes #app (fc: appfn_call app{correct fc})
+  = let fn = appfn fc.fid_c in
+    let _,_,ws = fn fc.arg_c fc.inp_c in
+    ws
+
+(* does a function call reference a specific app key *)
+let refs #app (fc: appfn_call app) (k: app_key app.adm)
+  = let open FStar.Seq in
+  exists i. (let k',v = index fc.inp_c i in k = k')
+
+(* for a referenced key, return the parameter position index *)
+val refkey_idx (#app:_) (fc: appfn_call app) (k: app_key app.adm{fc `refs` k})
+  : i:_{let k',v = FStar.Seq.index fc.inp_c i in k' = k}
+
+(* the written-value of a key *)
+let write #app (fc: appfn_call app{correct fc}) (k: app_key app.adm{fc `refs` k})
+  = let i = refkey_idx fc k in
+    let ws = writes fc in
+    let open FStar.Seq in
+    index ws i
+
+
+
+(* does a fncall succeed for a given state and input? *)
+let succeeds #app (fc: appfn_call app)
+  = Some? (simulate_step fc st)
+
+(* for a successful proc call, the state after applying the function *)
+let apply #app (fc: appfn_call app) (st: app_state app.adm {succeeds fc st})
+  = let Some (st, _) = simulate_step fc st in
+    st
+
+(* for a referenced key, the input value provided to the function invocation *)
+let refkey_inp_val (#app:_) (fc: appfn_call app) (k: app_key app.adm{fc `refs` k})
+  = let open FStar.Seq in
+    let i = refkey_idx fc k in
+    let _,v = index fc.inp_c i in
+    v
+
+(* if a function application succeeds, then the input value provided as input for a key is consistent
+ * with the "pre" state *)
+val lemma_refkey_pre_val (#app:_)
+  (fc: appfn_call app)
+  (st: app_state app.adm)
+  (k: app_key app.adm{fc `refs` k})
+  : Lemma (requires (succeeds fc st))
+          (ensures (refkey_inp_val fc k = st k))
+
+let refkey_post_val #app (fc: appfn_call app) (k: _{fc `refs` k})
+  = let fn = appfn fc.fid_c in
+    let rc
